proofs/isqrt_lean4/IsqrtTests.lean
@@ -1,3 +1,4 @@
 import Isqrt.Tests.PythonOps
 import Isqrt.Tests.Isqrt
 import Isqrt.Tests.While
+import Isqrt.Tests.Iterative
